

# Solved selected problems of Calculus on Manifolds by Michael Spivak

Franco Zacco

## 2 - Differentiation

### Basic Definitions

*Proof. 2-2.* Let  $f : \mathbb{R}^2 \rightarrow \mathbb{R}$  be independent of the second variable i.e. for each  $x \in \mathbb{R}$  we have that  $f(x, y_1) = f(x, y_2)$  for all  $y_1, y_2 \in \mathbb{R}$ .

Then we can take some  $y_0 \in \mathbb{R}$  and define a function  $g : \mathbb{R} \rightarrow \mathbb{R}$  such that  $g(x) = f(x, y_0)$ , then, for any  $y \in \mathbb{R}$  we get that  $f(x, y) = f(x, y_0) = g(x)$  because  $f$  is independent of the second variable.

On the other hand, suppose we have a function  $g : \mathbb{R} \rightarrow \mathbb{R}$  such that  $g(x) = f(x, y)$  then since this is true for any  $y \in \mathbb{R}$  then we can write that

$$f(x, y_1) = g(x) = f(x, y_2)$$

for any  $y_1, y_2 \in \mathbb{R}$ , which implies that  $f$  is independent of the second variable.

The Jacobian of  $f$  at  $(a, b)$  i.e.  $f'(a, b)$  is given by

$$f'(a, b) = (D_1f(a, b), D_2f(a, b))$$

Since  $g(x) = f(x, y)$  then  $D_1f(a, b) = D_1g(a) = g'(a)$  therefore

$$f'(a, b) = (g'(a), 0)$$

□

*Proof. 2-3.* A function  $f : \mathbb{R}^2 \rightarrow \mathbb{R}$  is independent of the first variable if for each  $y \in \mathbb{R}$  we have that  $f(x_1, y) = f(x_2, y)$  for all  $x_1, x_2 \in \mathbb{R}$ .

The Jacobian  $f'(a, b)$  in this case is

$$f'(a, b) = (D_1f(a, b), D_2f(a, b)) = (0, D_2f(a, b))$$

In the same way as we did in problem 2-2, we can show that  $f$  is independent of the first variable if and only if there is a function  $g : \mathbb{R} \rightarrow \mathbb{R}$  such that  $g(y) = f(x, y)$ .

So we get that  $D_2f(a, b) = D_2g(b) = g'(b)$  and therefore

$$f'(a, b) = (0, g'(b))$$

Finally, the functions that are independent of the first and the second variable are the functions of the form  $f(x, y) = c$  where  $c$  is a constant.  $\square$

*Proof. 2-4.* Let us define  $f : \mathbb{R}^2 \rightarrow \mathbb{R}$  by

$$f(x) = \begin{cases} |x| \cdot g\left(\frac{x}{|x|}\right) & x \neq 0 \\ 0 & x = 0 \end{cases}$$

Where  $g$  is a continuous real-valued function on the unit circle  $\{x \in \mathbb{R}^2 : |x| = 1\}$  such that  $g(0, 1) = g(1, 0) = 0$  and  $g(-x) = -g(x)$ .

(a) If  $x \in \mathbb{R}^2$  and  $h : \mathbb{R} \rightarrow \mathbb{R}$  defined by  $h(t) = f(tx)$ , we want to show that  $h$  is differentiable.

Suppose  $x \neq 0$ , also, let  $a \in \mathbb{R}$  and let  $\lambda(k) = k|x|g\left(\frac{x}{|x|}\right)$  then

$$\begin{aligned} \lim_{k \rightarrow 0} \frac{|h(a+k) - h(a) - \lambda(k)|}{|k|} &= \lim_{k \rightarrow 0} \frac{|f((a+k)x) - f(ax) - \lambda(k)|}{|k|} = \\ &= \lim_{k \rightarrow 0} \frac{1}{|k|} \left| |(a+k)x|g\left(\frac{(a+k)x}{|(a+k)x|}\right) - |ax|g\left(\frac{ax}{|ax|}\right) - k|x|g\left(\frac{x}{|x|}\right) | \right| \end{aligned}$$

Suppose  $a+k > 0$ , and suppose  $a > 0$  then

$$\begin{aligned} &\frac{1}{|k|} \left| |(a+k)x|g\left(\frac{(a+k)x}{|(a+k)x|}\right) - |ax|g\left(\frac{ax}{|ax|}\right) - k|x|g\left(\frac{x}{|x|}\right) | \right| = \\ &= \frac{1}{|k|} \left| (a+k)|x|g\left(\frac{x}{|x|}\right) - a|x|g\left(\frac{x}{|x|}\right) - k|x|g\left(\frac{x}{|x|}\right) | \right| \\ &= 0 \end{aligned}$$

If  $a < 0$  then

$$|ax|g\left(\frac{ax}{|ax|}\right) = -a|x|g\left(-\frac{ax}{a|x|}\right) = a|x|g\left(\frac{x}{|x|}\right)$$

Where we used that  $g(-x) = -g(x)$  and hence

$$\begin{aligned} &\frac{1}{|k|} \left| |(a+k)x|g\left(\frac{(a+k)x}{|(a+k)x|}\right) - |ax|g\left(\frac{ax}{|ax|}\right) - k|x|g\left(\frac{x}{|x|}\right) | \right| = \\ &= \frac{1}{|k|} \left| (a+k)|x|g\left(\frac{x}{|x|}\right) - a|x|g\left(\frac{x}{|x|}\right) - k|x|g\left(\frac{x}{|x|}\right) | \right| \\ &= 0 \end{aligned}$$

Now suppose  $a+k < 0$  then

$$\begin{aligned} &\frac{1}{|k|} \left| |(a+k)x|g\left(\frac{(a+k)x}{|(a+k)x|}\right) - |ax|g\left(\frac{ax}{|ax|}\right) - k|x|g\left(\frac{x}{|x|}\right) | \right| = \\ &= \left| -(a+k)|x|g\left(-\frac{(a+k)x}{(a+k)|x|}\right) - a|x|g\left(\frac{x}{|x|}\right) - k|x|g\left(\frac{x}{|x|}\right) \right| \\ &= \left| (a+k)|x|g\left(\frac{x}{|x|}\right) - a|x|g\left(\frac{x}{|x|}\right) - k|x|g\left(\frac{x}{|x|}\right) \right| \\ &= 0 \end{aligned}$$

Finally if  $a + k = 0$

$$\begin{aligned} & \frac{1}{|k|} \left| |(a+k)x|g\left(\frac{(a+k)x}{|(a+k)x|}\right) - |ax|g\left(\frac{ax}{|ax|}\right) - k|x|g\left(\frac{x}{|x|}\right) \right| = \\ &= \frac{1}{|k|} \left| k|x|g\left(\frac{ax}{|ax|}\right) - k|x|g\left(\frac{x}{|x|}\right) \right| \\ &= 0 \end{aligned}$$

In the case  $x = 0$  we see that  $\lambda(k) = 0$  and hence

$$\begin{aligned} & \frac{1}{|k|} \left| |(a+k)x|g\left(\frac{(a+k)x}{|(a+k)x|}\right) - |ax|g\left(\frac{ax}{|ax|}\right) - k|x|g\left(\frac{x}{|x|}\right) \right| = \\ &= \frac{1}{|k|} \left| 0 - 0 - 0 \right| \\ &= 0 \end{aligned}$$

Therefore  $h$  is differentiable.

(b) Let us compute  $Df(0,0)$  as follows

$$\begin{aligned} & \lim_{(h,k) \rightarrow (0,0)} \frac{|f(0+(h,k)) - f(0) - Df(0,0)(h,k)|}{|(h,k)|} \\ &= \lim_{(h,k) \rightarrow (0,0)} \frac{1}{|(h,k)|} \left| |(h,k)|g\left(\frac{(h,k)}{|(h,k)|}\right) - Df(0,0)(h,k) \right| \end{aligned}$$

Let  $h = 0$  then

$$\begin{aligned} & \frac{1}{|(0,k)|} \left| |(0,k)|g\left(\frac{(0,k)}{|(0,k)|}\right) - Df(0,0)(0,k) \right| \\ &= \frac{1}{|k|} \left| |k|g\left(0, \frac{k}{|k|}\right) - D_2f(0,0)k \right| \\ &\leq \frac{1}{|k|} \left| |k|g\left(0, \frac{k}{|k|}\right) \right| + \frac{1}{|k|} \left| D_2f(0,0)k \right| \\ &= \left| g\left(0, \frac{k}{|k|}\right) \right| + \left| D_2f(0,0) \right| \end{aligned}$$

We see that  $g(0, k/|k|) = g(0, 1) = 0$  if  $k > 0$ , if  $k < 0$  then  $g(0, k/|k|) = g(0, -1) = g(-(0, 1)) = -g(0, 1) = 0$ , then we get that

$$0 \leq \frac{1}{|(0,k)|} \left| |(0,k)|g\left(\frac{(0,k)}{|(0,k)|}\right) - Df(0,0)(0,k) \right| \leq \left| D_2f(0,0) \right|$$

In the same way, if we let  $k = 0$  instead

$$\begin{aligned}
& \frac{1}{|(h, 0)|} \left| |(h, 0)| g\left(\frac{(h, 0)}{|(h, 0)|}\right) - Df(0, 0)(h, 0) \right| \\
&= \frac{1}{|h|} \left| |h| g\left(\frac{h}{|h|}, 0\right) - D_1 f(0, 0)h \right| \\
&\leq \frac{1}{|h|} \left| |h| g\left(\frac{h}{|h|}, 0\right) \right| + \frac{1}{|h|} \left| D_1 f(0, 0)h \right| \\
&= \left| g\left(\frac{h}{|h|}, 0\right) \right| + \left| D_1 f(0, 0) \right|
\end{aligned}$$

Then since  $g(0, 1) = 0$  we get that

$$0 \leq \frac{1}{|(h, 0)|} \left| |(h, 0)| g\left(\frac{(h, 0)}{|(h, 0)|}\right) - Df(0, 0)(h, 0) \right| \leq \left| D_1 f(0, 0) \right|$$

Therefore must be that  $Df(0, 0) = 0$  for the limit

$$\lim_{(h, k) \rightarrow (0, 0)} \frac{|f(0 + (h, k)) - f(0) - Df(0, 0)(h, k)|}{|(h, k)|}$$

to converge to 0.

Then for any path taken by  $h$  and  $k$  the limit becomes

$$\begin{aligned}
& \lim_{(h, k) \rightarrow (0, 0)} \frac{|f(0 + (h, k)) - f(0) - Df(0, 0)(h, k)|}{|(h, k)|} \\
&= \lim_{(h, k) \rightarrow (0, 0)} \frac{1}{|(h, k)|} \left| |(h, k)| g\left(\frac{(h, k)}{|(h, k)|}\right) - 0 \right| \\
&= \lim_{(h, k) \rightarrow (0, 0)} \left| g\left(\frac{(h, k)}{|(h, k)|}\right) \right|
\end{aligned}$$

But  $g$  is only defined at the unit circle so this limit can only be 0 if  $g = 0$  and hence  $f$  is not continuous at  $(0, 0)$ .

□

*Proof. 2-5.* Let  $f : \mathbb{R}^2 \rightarrow \mathbb{R}$  be defined by

$$f(x, y) = \begin{cases} \frac{x|y|}{\sqrt{x^2+y^2}} & (x, y) \neq 0 \\ 0 & (x, y) = 0 \end{cases}$$

We can write that

$$\frac{x|y|}{\sqrt{x^2+y^2}} = \sqrt{x^2+y^2} \cdot \frac{x|y|}{x^2+y^2} = |(x, y)| \cdot \frac{x|y|}{|(x, y)|^2}$$

Then defining  $g$  as  $g(x, y) = x|y|$  we see that

$$g\left(\frac{(x, y)}{|(x, y)|}\right) = \frac{x}{|(x, y)|} \left| \frac{y}{|(x, y)|} \right| = \frac{x|y|}{|(x, y)|^2}$$

Also, we see that  $g(0, 1) = g(1, 0) = 0$  and that

$$g(-x, -y) = -x|-y| = -xy = -x|y| = -g(x, y)$$

Hence we can write  $f(x, y)$  as

$$f(x, y) = \begin{cases} |(x, y)| \cdot g\left(\frac{(x, y)}{|(x, y)|}\right) & (x, y) \neq 0 \\ 0 & (x, y) = 0 \end{cases}$$

Where  $g$  is a continuous real-valued function with the same properties described in Problem 2-4.

Therefore we can conclude that  $f$  is not differentiable at  $(0, 0)$ .  $\square$

*Proof. 2-6.* Let  $f : \mathbb{R}^2 \rightarrow \mathbb{R}$  be defined by  $f(x, y) = \sqrt{|xy|}$ , we may also define  $f$  as

$$f(x, y) = \begin{cases} \frac{\sqrt{x^2+y^2}\sqrt{|xy|}}{\sqrt{x^2+y^2}} & (x, y) \neq 0 \\ 0 & (x, y) = 0 \end{cases}$$

We see that

$$\frac{\sqrt{x^2+y^2}\sqrt{|xy|}}{\sqrt{x^2+y^2}} = |(x, y)| \frac{\sqrt{|xy|}}{|(x, y)|}$$

We can define a function  $g$  as  $g(x, y) = \sqrt{|xy|}$  so

$$g\left(\frac{(x, y)}{|(x, y)|}\right) = \sqrt{\left|\frac{x}{|(x, y)|} \frac{y}{|(x, y)|}\right|} = \sqrt{\frac{|xy|}{|(x, y)|^2}} = \frac{\sqrt{|xy|}}{|(x, y)|}$$

Also, we see that  $g(0, 1) = g(1, 0) = 0$  and that

$$g(-x, -y) = \pm\sqrt{|(-x)(-y)|} = \pm\sqrt{|xy|} = \pm g(x, y)$$

Hence we can write  $f(x, y)$  as

$$f(x, y) = \begin{cases} |(x, y)| \cdot g\left(\frac{(x, y)}{|(x, y)|}\right) & (x, y) \neq 0 \\ 0 & (x, y) = 0 \end{cases}$$

Where  $g$  is a continuous real-valued function with the same properties described in Problem 2-4.

Therefore we can conclude that  $f$  is not differentiable at  $(0, 0)$ . □

*Proof. 2-7.* Let  $f : \mathbb{R}^n \rightarrow \mathbb{R}$  be a function such that  $|f(x)| \leq |x|^2$  we want to show that  $f$  is differentiable at 0.

Let us consider the following limit

$$\lim_{h \rightarrow 0} \frac{|f(0+h) - f(0) - Df(0)h|}{|h|}$$

We see that

$$\begin{aligned} 0 \leq \frac{|f(0+h) - f(0) - Df(0)h|}{|h|} &\leq \frac{|f(h)| + |f(0)| + |Df(0)h|}{|h|} \\ &\leq \frac{|h|^2 + 0 + |Df(0)||h|}{|h|} \\ &\leq |h| + |Df(0)| \end{aligned}$$

We see that  $|h| + |Df(0)| \rightarrow 0$  as  $h \rightarrow 0$  if  $Df(0) = 0$ .

Therefore  $f$  is differentiable at 0. □



## Basic Theorems